Wrote up heap memory and conversion

08HeapMemory/HeapConversion.thy
@@ -2,39 +2,37 @@ theory HeapConversion
   imports HeapMemory
 begin
 
-primrec stack_below :: "ptr \<Rightarrow> ptr list \<Rightarrow> bool" where
-  "stack_below x [] = True"
-| "stack_below x (v # vs) = (v < x \<and> stack_below x vs)"
+subsection \<open>Heap conversion\<close>
 
-lemma [simp]: "stack_below x ys \<Longrightarrow> y \<in> set ys \<Longrightarrow> y < x"
-  by (induction ys) auto
+text \<open>As usual with evaluation state refinements, many possible heaps correspond to one bytecode 
+state. So we must define our conversion functions running backwards; taking care to make sure that 
+each function terminates. Unlike the codebase ordered-pointer property, which could be falsified by
+looping code or other features we carefully avoid, the ordered-heap property we use here is 
+necessarily true even for a more complex language, since no value, no matter what kind, can 
+reference values that haven't even been allocated yet.\<close>
 
-fun unheap_closure :: "hclosure heap \<Rightarrow> ptr \<Rightarrow> closure\<^sub>b" where
+fun unheap_closure :: "closure\<^sub>h heap \<Rightarrow> ptr \<Rightarrow> closure\<^sub>b" where
   "unheap_closure h x = (case hlookup h x of 
-      HConst k \<Rightarrow> Const\<^sub>b k
-    | HLam env pc \<Rightarrow> 
-        Lam\<^sub>b (if stack_below x env then map (unheap_closure h) env else undefined) pc)"
+      Const\<^sub>h n \<Rightarrow> Const\<^sub>b n
+    | Lam\<^sub>h \<Delta> p \<Rightarrow> Lam\<^sub>b (if list_all ((>) x) \<Delta> then map (unheap_closure h) \<Delta> else undefined) p)"
 
-fun unheap_stack :: "hclosure heap \<Rightarrow> (ptr list \<times> nat) list \<Rightarrow> (closure\<^sub>b list \<times> nat) list" where
-  "unheap_stack h [] = []"
-| "unheap_stack h ((env, pc) # sfs) = ((map (unheap_closure h) env, pc) # unheap_stack h sfs)"
+abbreviation unheap_stack :: "closure\<^sub>h heap \<Rightarrow> (ptr list \<times> nat) list \<Rightarrow> (closure\<^sub>b list \<times> nat) list" 
+    where
+  "unheap_stack h s \<equiv> map (\<lambda>(\<Delta>, p). (map (unheap_closure h) \<Delta>, p)) s"
 
 primrec unheap :: "heap_state \<Rightarrow> state\<^sub>b" where
-  "unheap (HS h vs sfs) = S\<^sub>b (map (unheap_closure h) vs) (unheap_stack h sfs)"
+  "unheap (S\<^sub>h h \<V> s) = S\<^sub>b (map (unheap_closure h) \<V>) (unheap_stack h s)"
 
-primrec bounded_closure :: "hclosure heap \<Rightarrow> ptr \<Rightarrow> hclosure \<Rightarrow> bool" where
-  "bounded_closure h x (HConst k) = True"
-| "bounded_closure h x (HLam env pc) = (list_all (hcontains h) env \<and> stack_below x env)"
+primrec bounded_closure :: "closure\<^sub>h heap \<Rightarrow> ptr \<Rightarrow> closure\<^sub>h \<Rightarrow> bool" where
+  "bounded_closure h x (Const\<^sub>h n) = True"
+| "bounded_closure h x (Lam\<^sub>h \<Delta> p) = (list_all (hcontains h) \<Delta> \<and> list_all ((>) x) \<Delta>)"
 
-primrec heap_structured :: "heap_state \<Rightarrow> bool" where
-  "heap_structured (HS h vs sfs) = (heap_all (bounded_closure h) h \<and>
-    list_all (hcontains h) vs \<and> list_all (list_all (hcontains h)) (map fst sfs))"
-
-lemma [simp]: "halloc h a = (h', x) \<Longrightarrow> bounded_closure h y c \<Longrightarrow> bounded_closure h' y c"
+lemma halloc_bounded [simp]: "halloc h a = (h', x) \<Longrightarrow> bounded_closure h y c \<Longrightarrow> 
+    bounded_closure h' y c"
   by (induction c) simp_all
 
-lemma [simp]: "heap_all (bounded_closure h) h \<Longrightarrow> halloc h c = (h', v) \<Longrightarrow> bounded_closure h v c \<Longrightarrow> 
-    heap_all (bounded_closure h') h'"
+lemma halloc_heap_bounded [simp]: "heap_all (bounded_closure h) h \<Longrightarrow> halloc h c = (h', v) \<Longrightarrow> 
+  bounded_closure h v c \<Longrightarrow> heap_all (bounded_closure h') h'"
 proof -
   assume A: "halloc h c = (h', v)" and "heap_all (bounded_closure h) h" and "bounded_closure h v c"
   hence "heap_all (bounded_closure h) h'" by auto
@@ -42,157 +40,151 @@ proof -
   ultimately show ?thesis by auto
 qed
 
-lemma [simp]: "halloc h (HConst k) = (h', v) \<Longrightarrow> unheap_closure h' v = Const\<^sub>b k"
-  by simp
-
-lemma [simp]: "halloc h c = (h', v) \<Longrightarrow> list_all (hcontains h) env \<Longrightarrow> stack_below v env"
-  by (induction env) simp_all
-
-lemma [simp]: "halloc h c = (h', v) \<Longrightarrow> hcontains h x \<Longrightarrow> heap_all (bounded_closure h) h \<Longrightarrow> 
-  unheap_closure h' x = unheap_closure h x"
+lemma halloc_unheap_closure [simp]: "halloc h c = (h', v) \<Longrightarrow> hcontains h x \<Longrightarrow> 
+  heap_all (bounded_closure h) h \<Longrightarrow> unheap_closure h' x = unheap_closure h x"
 proof (induction h x rule: unheap_closure.induct)
   case (1 h x)
   thus ?case
   proof (cases "hlookup h x")
-    case (HLam env p)
+    case (Lam\<^sub>h \<Delta> p)
     with 1 show ?thesis
-    proof (cases "stack_below x env")
+    proof (cases "list_all ((>) x) \<Delta>")
       case True
-      from HLam 1 have "list_all (hcontains h) env" by (metis hlookup_all bounded_closure.simps(2))
-      hence S: "\<And>y. y \<in> set env \<Longrightarrow> hcontains h y" by auto
-      from 1 HLam True have "\<And>y. y \<in> set env \<Longrightarrow> hcontains h y \<Longrightarrow> 
+      from Lam\<^sub>h 1 have "list_all (hcontains h) \<Delta>" by (metis hlookup_all bounded_closure.simps(2))
+      hence S: "\<And>y. y \<in> set \<Delta> \<Longrightarrow> hcontains h y" by auto
+      from 1 Lam\<^sub>h True have "\<And>y. y \<in> set \<Delta> \<Longrightarrow> hcontains h y \<Longrightarrow> 
         unheap_closure h' y = unheap_closure h y" by simp
-      with S 1(2, 3) HLam True show ?thesis by simp
+      with S 1(2, 3) Lam\<^sub>h True show ?thesis by simp
     qed simp_all
   qed simp_all
 qed
 
-lemma [simp]: "halloc h c = (h', v) \<Longrightarrow> list_all (hcontains h) env \<Longrightarrow> heap_all (bounded_closure h) h \<Longrightarrow>
-    map (unheap_closure h') env = map (unheap_closure h) env"
-  by (induction env) (simp_all del: unheap_closure.simps)
+lemma halloc_unheap_env [simp]: "halloc h c = (h', v) \<Longrightarrow> list_all (hcontains h) \<Delta> \<Longrightarrow> 
+    heap_all (bounded_closure h) h \<Longrightarrow> map (unheap_closure h') \<Delta> = map (unheap_closure h) \<Delta>"
+  by (induction \<Delta>) (simp_all del: unheap_closure.simps)
 
-lemma [simp]: "halloc h c = (h', v) \<Longrightarrow> list_all (list_all (hcontains h)) (map fst sfs) \<Longrightarrow> 
-    heap_all (bounded_closure h) h \<Longrightarrow> unheap_stack h' sfs = unheap_stack h sfs"
-  by (induction sfs rule: unheap_stack.induct) (simp_all del: unheap_closure.simps)
+lemma halloc_unheap_stack [simp]: "halloc h c = (h', v) \<Longrightarrow> 
+  list_all (list_all (hcontains h)) (map fst s) \<Longrightarrow> heap_all (bounded_closure h) h \<Longrightarrow> 
+    unheap_stack h' s = unheap_stack h s"
+  by (induction s) (auto simp del: unheap_closure.simps)
 
-lemma [simp]: "halloc h (HLam env p) = (h', v) \<Longrightarrow> list_all (hcontains h) env \<Longrightarrow> 
-    heap_all (bounded_closure h) h \<Longrightarrow> unheap_closure h' v = Lam\<^sub>b (map (unheap_closure h) env) p"
-  by simp
-
-lemma [simp]: "hlookup h v = HLam env pc \<Longrightarrow> heap_all (bounded_closure h) h \<Longrightarrow> hcontains h v \<Longrightarrow>
-    stack_below v env"
+lemma hlookup_lam_bounded [simp]: "hlookup h v = Lam\<^sub>h \<Delta> p \<Longrightarrow> heap_all (bounded_closure h) h \<Longrightarrow> 
+    hcontains h v \<Longrightarrow> list_all ((>) v) \<Delta>"
   by (metis hlookup_all bounded_closure.simps(2))
 
-lemma [simp]: "cd \<tturnstile> \<Sigma>\<^sub>h \<leadsto>\<^sub>h \<Sigma>\<^sub>h' \<Longrightarrow> heap_structured \<Sigma>\<^sub>h \<Longrightarrow> heap_structured \<Sigma>\<^sub>h'"
-proof (induction \<Sigma>\<^sub>h \<Sigma>\<^sub>h' rule: evalh.induct)
-  case (evh_apply cd pc h v2 env pc' v1 vs sfs)
-  hence "hlookup h v2 = HLam env pc' \<and> heap_all (bounded_closure h) h \<and> hcontains h v2" by simp
-  hence "bounded_closure h v2 (HLam env pc')" by (metis hlookup_all)
-  with evh_apply show ?case by simp
+primrec heap_structured :: "heap_state \<Rightarrow> bool" where
+  "heap_structured (S\<^sub>h h \<V> s) = (heap_all (bounded_closure h) h \<and>
+    list_all (hcontains h) \<V> \<and> list_all (list_all (hcontains h)) (map fst s))"
+
+lemma eval_heap_structured [simp]: "\<C> \<tturnstile> \<Sigma>\<^sub>h \<leadsto>\<^sub>h \<Sigma>\<^sub>h' \<Longrightarrow> heap_structured \<Sigma>\<^sub>h \<Longrightarrow> heap_structured \<Sigma>\<^sub>h'"
+proof (induction \<Sigma>\<^sub>h \<Sigma>\<^sub>h' rule: eval\<^sub>h.induct)
+  case (ev\<^sub>h_apply \<C> p h v\<^sub>2 \<Delta> p' v\<^sub>1 \<V> s)
+  hence "hlookup h v\<^sub>2 = Lam\<^sub>h \<Delta> p' \<and> heap_all (bounded_closure h) h \<and> hcontains h v\<^sub>2" by simp
+  hence "bounded_closure h v\<^sub>2 (Lam\<^sub>h \<Delta> p')" by (metis hlookup_all)
+  with ev\<^sub>h_apply show ?case by simp
 next
-  case (evh_jump cd pc h v2 env' pc' v1 vs env sfs)
-  hence "hlookup h v2 = HLam env' pc' \<and> heap_all (bounded_closure h) h \<and> hcontains h v2" by simp
-  hence "bounded_closure h v2 (HLam env' pc')" by (metis hlookup_all)
-  with evh_jump show ?case by simp
+  case (ev\<^sub>h_jump \<C> p h v\<^sub>2 \<Delta>' p' v\<^sub>1 \<V> \<Delta> s)
+  hence "hlookup h v\<^sub>2 = Lam\<^sub>h \<Delta>' p' \<and> heap_all (bounded_closure h) h \<and> hcontains h v\<^sub>2" by simp
+  hence "bounded_closure h v\<^sub>2 (Lam\<^sub>h \<Delta>' p')" by (metis hlookup_all)
+  with ev\<^sub>h_jump show ?case by simp
 qed fastforce+
 
-lemma [simp]: "iter (\<tturnstile> cd \<leadsto>\<^sub>h) \<Sigma>\<^sub>h \<Sigma>\<^sub>h' \<Longrightarrow> heap_structured \<Sigma>\<^sub>h \<Longrightarrow> heap_structured \<Sigma>\<^sub>h'"
-  by (induction \<Sigma>\<^sub>h \<Sigma>\<^sub>h' rule: iter.induct) simp_all
+text \<open>The completeness proof is our most straightforward yet.\<close>
 
-theorem correcth [simp]: "cd \<tturnstile> \<Sigma>\<^sub>h \<leadsto>\<^sub>h \<Sigma>\<^sub>h' \<Longrightarrow> heap_structured \<Sigma>\<^sub>h \<Longrightarrow> cd \<tturnstile> unheap \<Sigma>\<^sub>h \<leadsto>\<^sub>b unheap \<Sigma>\<^sub>h'"
-  by (induction \<Sigma>\<^sub>h \<Sigma>\<^sub>h' rule: evalh.induct) simp_all
+theorem complete\<^sub>h [simp]: "\<C> \<tturnstile> \<Sigma>\<^sub>h \<leadsto>\<^sub>h \<Sigma>\<^sub>h' \<Longrightarrow> heap_structured \<Sigma>\<^sub>h \<Longrightarrow> \<C> \<tturnstile> unheap \<Sigma>\<^sub>h \<leadsto>\<^sub>b unheap \<Sigma>\<^sub>h'"
+  by (induction \<Sigma>\<^sub>h \<Sigma>\<^sub>h' rule: eval\<^sub>h.induct) simp_all
 
-lemma [simp]: "S\<^sub>b vs ((env, pc) # sfs) = unheap \<Sigma>\<^sub>h \<Longrightarrow> \<exists>h vs' env' sfs'. 
-  \<Sigma>\<^sub>h = HS h vs' ((env', pc) # sfs') \<and> vs = map (unheap_closure h) vs' \<and> 
-    env = map (unheap_closure h) env' \<and> sfs = unheap_stack h sfs'"
+text \<open>But even correctness isn't too bad.\<close>
+
+lemma unheap_to_empty [simp]: "S\<^sub>b \<V>\<^sub>b [] = unheap \<Sigma>\<^sub>h \<Longrightarrow> \<exists>h \<V>\<^sub>h. 
+  \<Sigma>\<^sub>h = S\<^sub>h h \<V>\<^sub>h [] \<and> \<V>\<^sub>b = map (unheap_closure h) \<V>\<^sub>h"
 proof (induction \<Sigma>\<^sub>h)
-  case (HS h vs' sfs')
-  thus ?case by (induction h sfs' rule: unheap_stack.induct) (simp_all del: unheap_closure.simps)
+  case (S\<^sub>h h \<V>\<^sub>h s\<^sub>h)
+  thus ?case by (induction s\<^sub>h) (simp_all del: unheap_closure.simps)
 qed 
 
-lemma unheap_empty [simp]: "S\<^sub>b vs [] = unheap \<Sigma>\<^sub>h \<Longrightarrow> \<exists>h vs'. 
-  \<Sigma>\<^sub>h = HS h vs' [] \<and> vs = map (unheap_closure h) vs'"
+lemma unheap_to_cons [simp]: "S\<^sub>b \<V>\<^sub>b ((\<Delta>, p) # s) = unheap \<Sigma>\<^sub>h \<Longrightarrow> \<exists>h \<V>\<^sub>h \<Delta>\<^sub>h s\<^sub>h. 
+  \<Sigma>\<^sub>h = S\<^sub>h h \<V>\<^sub>h ((\<Delta>\<^sub>h, p) # s\<^sub>h) \<and> \<V>\<^sub>b = map (unheap_closure h) \<V>\<^sub>h \<and> 
+    \<Delta> = map (unheap_closure h) \<Delta>\<^sub>h \<and> s = unheap_stack h s\<^sub>h"
 proof (induction \<Sigma>\<^sub>h)
-  case (HS h vs' sfs')
-  thus ?case by (induction h sfs' rule: unheap_stack.induct) (simp_all del: unheap_closure.simps)
+  case (S\<^sub>h h \<V>\<^sub>h s\<^sub>h)
+  thus ?case by (induction s\<^sub>h) (auto simp del: unheap_closure.simps)
 qed 
 
-lemma [simp]: "unheap_closure h v = Lam\<^sub>b env pc \<Longrightarrow> hcontains h v \<Longrightarrow> 
+lemma unheap_to_lam [simp]: "unheap_closure h v = Lam\<^sub>b \<Delta>\<^sub>b p \<Longrightarrow> hcontains h v \<Longrightarrow> 
   heap_all (bounded_closure h) h \<Longrightarrow> 
-    \<exists>env'. hlookup h v = HLam env' pc \<and> env = map (unheap_closure h) env'"
-  by (simp split: hclosure.splits if_splits)
+    \<exists>\<Delta>\<^sub>h. hlookup h v = Lam\<^sub>h \<Delta>\<^sub>h p \<and> \<Delta>\<^sub>b = map (unheap_closure h) \<Delta>\<^sub>h"
+  by (simp split: closure\<^sub>h.splits if_splits)
 
-theorem completeh [simp]: "cd \<tturnstile> unheap \<Sigma>\<^sub>h \<leadsto>\<^sub>b \<Sigma>\<^sub>b' \<Longrightarrow> heap_structured \<Sigma>\<^sub>h \<Longrightarrow> 
-  \<exists>\<Sigma>\<^sub>h'. (cd \<tturnstile> \<Sigma>\<^sub>h \<leadsto>\<^sub>h \<Sigma>\<^sub>h') \<and> \<Sigma>\<^sub>b' = unheap \<Sigma>\<^sub>h'"
+theorem correct\<^sub>h [simp]: "\<C> \<tturnstile> unheap \<Sigma>\<^sub>h \<leadsto>\<^sub>b \<Sigma>\<^sub>b' \<Longrightarrow> heap_structured \<Sigma>\<^sub>h \<Longrightarrow> 
+  \<exists>\<Sigma>\<^sub>h'. (\<C> \<tturnstile> \<Sigma>\<^sub>h \<leadsto>\<^sub>h \<Sigma>\<^sub>h') \<and> \<Sigma>\<^sub>b' = unheap \<Sigma>\<^sub>h'"
 proof (induction "unheap \<Sigma>\<^sub>h" \<Sigma>\<^sub>b' rule: eval\<^sub>b.induct)
-  case (ev\<^sub>b_lookup cd pc x env v vs sfs)
-  then obtain h vs' env' sfs' where "\<Sigma>\<^sub>h = HS h vs' ((env', Suc pc) # sfs') \<and> 
-    vs = map (unheap_closure h) vs' \<and> env = map (unheap_closure h) env' \<and> sfs = unheap_stack h sfs'" 
-      by fastforce
-  moreover with ev\<^sub>b_lookup obtain vv where "lookup env' x = Some vv \<and> v = unheap_closure h vv" 
+  case (ev\<^sub>b_lookup \<C> p x \<Delta>\<^sub>b v \<V>\<^sub>b s\<^sub>b)
+  then obtain h \<V>\<^sub>h \<Delta>\<^sub>h s\<^sub>h where "\<Sigma>\<^sub>h = S\<^sub>h h \<V>\<^sub>h ((\<Delta>\<^sub>h, Suc p) # s\<^sub>h) \<and> \<V>\<^sub>b = map (unheap_closure h) \<V>\<^sub>h \<and> 
+    \<Delta>\<^sub>b = map (unheap_closure h) \<Delta>\<^sub>h \<and> s\<^sub>b = unheap_stack h s\<^sub>h" by fastforce
+  moreover with ev\<^sub>b_lookup obtain vv where "lookup \<Delta>\<^sub>h x = Some vv \<and> v = unheap_closure h vv" 
     by fastforce
-  moreover with ev\<^sub>b_lookup have "cd \<tturnstile> HS h vs' ((env', Suc pc) # sfs') \<leadsto>\<^sub>h 
-    HS h (vv # vs') ((env', pc) # sfs')" by simp
+  moreover with ev\<^sub>b_lookup have "\<C> \<tturnstile> S\<^sub>h h \<V>\<^sub>h ((\<Delta>\<^sub>h, Suc p) # s\<^sub>h) \<leadsto>\<^sub>h S\<^sub>h h (vv # \<V>\<^sub>h) ((\<Delta>\<^sub>h, p) # s\<^sub>h)" 
+    by simp
   ultimately show ?case by fastforce
 next
-  case (ev\<^sub>b_pushcon cd pc k vs env sfs)
-  moreover then obtain h vs' env' sfs' where "\<Sigma>\<^sub>h = HS h vs' ((env', Suc pc) # sfs') \<and> 
-    vs = map (unheap_closure h) vs' \<and> env = map (unheap_closure h) env' \<and> sfs = unheap_stack h sfs'" 
+  case (ev\<^sub>b_pushcon \<C> p n \<V>\<^sub>b \<Delta>\<^sub>b s\<^sub>b)
+  moreover then obtain h \<V>\<^sub>h \<Delta>\<^sub>h s\<^sub>h where "\<Sigma>\<^sub>h = S\<^sub>h h \<V>\<^sub>h ((\<Delta>\<^sub>h, Suc p) # s\<^sub>h) \<and> 
+    \<V>\<^sub>b = map (unheap_closure h) \<V>\<^sub>h \<and> \<Delta>\<^sub>b = map (unheap_closure h) \<Delta>\<^sub>h \<and> s\<^sub>b = unheap_stack h s\<^sub>h" 
       by fastforce
-  moreover obtain h' v where "halloc h (HConst k) = (h', v)" by fastforce
-  moreover with ev\<^sub>b_pushcon have "cd \<tturnstile> HS h vs' ((env', Suc pc) # sfs') \<leadsto>\<^sub>h 
-    HS h' (v # vs') ((env', pc) # sfs')" by simp
+  moreover obtain h' v where "halloc h (Const\<^sub>h n) = (h', v)" by fastforce
+  moreover with ev\<^sub>b_pushcon have "\<C> \<tturnstile> S\<^sub>h h \<V>\<^sub>h ((\<Delta>\<^sub>h, Suc p) # s\<^sub>h) \<leadsto>\<^sub>h S\<^sub>h h' (v # \<V>\<^sub>h) ((\<Delta>\<^sub>h, p) # s\<^sub>h)" 
+    by simp
   ultimately show ?case by fastforce
 next
-  case (ev\<^sub>b_pushlam cd pc pc' vs env sfs)
-  moreover then obtain h vs' env' sfs' where S: "\<Sigma>\<^sub>h = HS h vs' ((env', Suc pc) # sfs') \<and> 
-    vs = map (unheap_closure h) vs' \<and> env = map (unheap_closure h) env' \<and> sfs = unheap_stack h sfs'" 
+  case (ev\<^sub>b_pushlam \<C> p p' \<V>\<^sub>b \<Delta>\<^sub>b s\<^sub>b)
+  moreover then obtain h \<V>\<^sub>h \<Delta>\<^sub>h s\<^sub>h where S: "\<Sigma>\<^sub>h = S\<^sub>h h \<V>\<^sub>h ((\<Delta>\<^sub>h, Suc p) # s\<^sub>h) \<and> 
+    \<V>\<^sub>b = map (unheap_closure h) \<V>\<^sub>h \<and> \<Delta>\<^sub>b = map (unheap_closure h) \<Delta>\<^sub>h \<and> s\<^sub>b = unheap_stack h s\<^sub>h" 
       by fastforce
-  moreover obtain h' v where "halloc h (HLam env' pc') = (h', v)" by fastforce
-  moreover with ev\<^sub>b_pushlam S have "cd \<tturnstile> HS h vs' ((env', Suc pc) # sfs') \<leadsto>\<^sub>h 
-    HS h' (v # vs') ((env', pc) # sfs')" by simp
+  moreover obtain h' v where "halloc h (Lam\<^sub>h \<Delta>\<^sub>h p') = (h', v)" by fastforce
+  moreover with ev\<^sub>b_pushlam S have "\<C> \<tturnstile> S\<^sub>h h \<V>\<^sub>h ((\<Delta>\<^sub>h, Suc p) # s\<^sub>h) \<leadsto>\<^sub>h S\<^sub>h h' (v # \<V>\<^sub>h) ((\<Delta>\<^sub>h, p) # s\<^sub>h)" 
+    by simp
   ultimately show ?case by fastforce
 next
-  case (ev\<^sub>b_apply cd pc v env' pc' vs env sfs)
-  then obtain h vs'' envh sfs' where S: "\<Sigma>\<^sub>h = HS h vs'' ((envh, Suc pc) # sfs') \<and> 
-    v # Lam\<^sub>b env' pc' # vs = map (unheap_closure h) vs'' \<and> env = map (unheap_closure h) envh \<and> 
-      sfs = unheap_stack h sfs'" by fastforce
-  moreover then obtain v1 v2 vs' where "vs'' = v1 # v2 # vs' \<and> v = unheap_closure h v1 \<and> 
-    Lam\<^sub>b env' pc' = unheap_closure h v2 \<and> vs = map (unheap_closure h) vs'" by fastforce
-  moreover with ev\<^sub>b_apply S obtain envh' where H: "hlookup h v2 = HLam envh' pc' \<and> 
-    env' = map (unheap_closure h) envh'" by fastforce
-  moreover with ev\<^sub>b_apply have "cd \<tturnstile> HS h (v1 # v2 # vs') ((envh, Suc pc) # sfs') \<leadsto>\<^sub>h 
-    HS h vs' ((v1 # envh', pc') # (envh, pc) # sfs')" by simp
+  case (ev\<^sub>b_apply \<C> p v\<^sub>b \<Delta>\<^sub>b' p' \<V>\<^sub>b \<Delta>\<^sub>b s\<^sub>b)
+  then obtain h \<V>\<^sub>h' \<Delta>\<^sub>h s\<^sub>h where S: "\<Sigma>\<^sub>h = S\<^sub>h h \<V>\<^sub>h' ((\<Delta>\<^sub>h, Suc p) # s\<^sub>h) \<and> 
+    v\<^sub>b # Lam\<^sub>b \<Delta>\<^sub>b' p' # \<V>\<^sub>b = map (unheap_closure h) \<V>\<^sub>h' \<and> \<Delta>\<^sub>b = map (unheap_closure h) \<Delta>\<^sub>h \<and> 
+      s\<^sub>b = unheap_stack h s\<^sub>h" by fastforce
+  moreover then obtain v\<^sub>h\<^sub>1 v\<^sub>h\<^sub>2 \<V>\<^sub>h where "\<V>\<^sub>h' = v\<^sub>h\<^sub>1 # v\<^sub>h\<^sub>2 # \<V>\<^sub>h \<and> v\<^sub>b = unheap_closure h v\<^sub>h\<^sub>1 \<and> 
+    Lam\<^sub>b \<Delta>\<^sub>b' p' = unheap_closure h v\<^sub>h\<^sub>2 \<and> \<V>\<^sub>b = map (unheap_closure h) \<V>\<^sub>h" by fastforce
+  moreover with ev\<^sub>b_apply S obtain \<Delta>h' where H: "hlookup h v\<^sub>h\<^sub>2 = Lam\<^sub>h \<Delta>h' p' \<and> 
+    \<Delta>\<^sub>b' = map (unheap_closure h) \<Delta>h'" by fastforce
+  moreover with ev\<^sub>b_apply have "\<C> \<tturnstile> S\<^sub>h h (v\<^sub>h\<^sub>1 # v\<^sub>h\<^sub>2 # \<V>\<^sub>h) ((\<Delta>\<^sub>h, Suc p) # s\<^sub>h) \<leadsto>\<^sub>h 
+    S\<^sub>h h \<V>\<^sub>h ((v\<^sub>h\<^sub>1 # \<Delta>h', p') # (\<Delta>\<^sub>h, p) # s\<^sub>h)" by simp
   ultimately show ?case by fastforce
 next
-  case (ev\<^sub>b_return cd pc vs env sfs)
-  then obtain h vs' env' sfs' where "\<Sigma>\<^sub>h = HS h vs' ((env', Suc pc) # sfs') \<and> 
-    vs = map (unheap_closure h) vs' \<and> env = map (unheap_closure h) env' \<and> sfs = unheap_stack h sfs'" 
-      by fastforce
-  moreover with ev\<^sub>b_return have "cd \<tturnstile> HS h vs' ((env', Suc pc) # sfs') \<leadsto>\<^sub>h HS h vs' sfs'" by simp
+  case (ev\<^sub>b_return \<C> p \<V>\<^sub>b \<Delta>\<^sub>b s\<^sub>b)
+  then obtain h \<V>\<^sub>h \<Delta>\<^sub>h s\<^sub>h where "\<Sigma>\<^sub>h = S\<^sub>h h \<V>\<^sub>h ((\<Delta>\<^sub>h, Suc p) # s\<^sub>h) \<and> \<V>\<^sub>b = map (unheap_closure h) \<V>\<^sub>h \<and> 
+    \<Delta>\<^sub>b = map (unheap_closure h) \<Delta>\<^sub>h \<and> s\<^sub>b = unheap_stack h s\<^sub>h" by fastforce
+  moreover with ev\<^sub>b_return have "\<C> \<tturnstile> S\<^sub>h h \<V>\<^sub>h ((\<Delta>\<^sub>h, Suc p) # s\<^sub>h) \<leadsto>\<^sub>h S\<^sub>h h \<V>\<^sub>h s\<^sub>h" by simp
   ultimately show ?case by fastforce
 next
-  case (ev\<^sub>b_jump cd pc v env' pc' vs env sfs)
-  then obtain h vs'' envh sfs' where S: "\<Sigma>\<^sub>h = HS h vs'' ((envh, Suc pc) # sfs') \<and> 
-    v # Lam\<^sub>b env' pc' # vs = map (unheap_closure h) vs'' \<and> env = map (unheap_closure h) envh \<and> 
-      sfs = unheap_stack h sfs'" by fastforce
-  moreover from S obtain v1 v2 vs' where "vs'' = v1 # v2 # vs' \<and> v = unheap_closure h v1 \<and> 
-    Lam\<^sub>b env' pc' = unheap_closure h v2 \<and> vs = map (unheap_closure h) vs'" by fastforce
-  moreover with ev\<^sub>b_jump S obtain envh' where "hlookup h v2 = HLam envh' pc' \<and> 
-    env' = map (unheap_closure h) envh'" by fastforce
-  moreover with ev\<^sub>b_jump S have "cd \<tturnstile> HS h (v1 # v2 # vs') ((envh, Suc pc) # sfs') \<leadsto>\<^sub>h 
-    HS h vs' ((v1 # envh', pc') # sfs')" by simp
+  case (ev\<^sub>b_jump \<C> p v\<^sub>b \<Delta>\<^sub>b' p' \<V>\<^sub>b \<Delta>\<^sub>b s\<^sub>b)
+  then obtain h \<V>\<^sub>h' \<Delta>\<^sub>h s\<^sub>h where S: "\<Sigma>\<^sub>h = S\<^sub>h h \<V>\<^sub>h' ((\<Delta>\<^sub>h, Suc p) # s\<^sub>h) \<and> 
+    v\<^sub>b # Lam\<^sub>b \<Delta>\<^sub>b' p' # \<V>\<^sub>b = map (unheap_closure h) \<V>\<^sub>h' \<and> \<Delta>\<^sub>b = map (unheap_closure h) \<Delta>\<^sub>h \<and> 
+      s\<^sub>b = unheap_stack h s\<^sub>h" by fastforce
+  moreover from S obtain v\<^sub>h\<^sub>1 v\<^sub>h\<^sub>2 \<V>\<^sub>h where "\<V>\<^sub>h' = v\<^sub>h\<^sub>1 # v\<^sub>h\<^sub>2 # \<V>\<^sub>h \<and> v\<^sub>b = unheap_closure h v\<^sub>h\<^sub>1 \<and> 
+    Lam\<^sub>b \<Delta>\<^sub>b' p' = unheap_closure h v\<^sub>h\<^sub>2 \<and> \<V>\<^sub>b = map (unheap_closure h) \<V>\<^sub>h" by fastforce
+  moreover with ev\<^sub>b_jump S obtain \<Delta>h' where "hlookup h v\<^sub>h\<^sub>2 = Lam\<^sub>h \<Delta>h' p' \<and> 
+    \<Delta>\<^sub>b' = map (unheap_closure h) \<Delta>h'" by fastforce
+  moreover with ev\<^sub>b_jump S have "\<C> \<tturnstile> S\<^sub>h h (v\<^sub>h\<^sub>1 # v\<^sub>h\<^sub>2 # \<V>\<^sub>h) ((\<Delta>\<^sub>h, Suc p) # s\<^sub>h) \<leadsto>\<^sub>h 
+    S\<^sub>h h \<V>\<^sub>h ((v\<^sub>h\<^sub>1 # \<Delta>h', p') # s\<^sub>h)" by simp
   ultimately show ?case by fastforce
 qed
 
-lemma [simp]: "iter (\<tturnstile> cd \<leadsto>\<^sub>b) (unheap \<Sigma>\<^sub>h) \<Sigma>\<^sub>b' \<Longrightarrow> heap_structured \<Sigma>\<^sub>h \<Longrightarrow> 
-  \<exists>\<Sigma>\<^sub>h'. iter (\<tturnstile> cd \<leadsto>\<^sub>h) \<Sigma>\<^sub>h \<Sigma>\<^sub>h' \<and> \<Sigma>\<^sub>b' = unheap \<Sigma>\<^sub>h'"
+lemma iter_correct\<^sub>h [simp]: "iter (\<tturnstile> \<C> \<leadsto>\<^sub>b) (unheap \<Sigma>\<^sub>h) \<Sigma>\<^sub>b' \<Longrightarrow> heap_structured \<Sigma>\<^sub>h \<Longrightarrow> 
+  \<exists>\<Sigma>\<^sub>h'. iter (\<tturnstile> \<C> \<leadsto>\<^sub>h) \<Sigma>\<^sub>h \<Sigma>\<^sub>h' \<and> \<Sigma>\<^sub>b' = unheap \<Sigma>\<^sub>h'"
 proof (induction "unheap \<Sigma>\<^sub>h" \<Sigma>\<^sub>b' arbitrary: \<Sigma>\<^sub>h rule: iter.induct)
   case (iter_step \<Sigma>\<^sub>b' \<Sigma>\<^sub>b'')
-  moreover then obtain \<Sigma>\<^sub>h' where S: "(cd \<tturnstile> \<Sigma>\<^sub>h \<leadsto>\<^sub>h \<Sigma>\<^sub>h') \<and> \<Sigma>\<^sub>b' = unheap \<Sigma>\<^sub>h'" by fastforce
+  moreover then obtain \<Sigma>\<^sub>h' where S: "(\<C> \<tturnstile> \<Sigma>\<^sub>h \<leadsto>\<^sub>h \<Sigma>\<^sub>h') \<and> \<Sigma>\<^sub>b' = unheap \<Sigma>\<^sub>h'" by fastforce
   moreover with iter_step have "heap_structured \<Sigma>\<^sub>h'" by fastforce
-  ultimately obtain \<Sigma>\<^sub>h'' where "iter (\<tturnstile> cd \<leadsto>\<^sub>h) \<Sigma>\<^sub>h' \<Sigma>\<^sub>h'' \<and> \<Sigma>\<^sub>b'' = unheap \<Sigma>\<^sub>h''" by fastforce
-  with S have "iter (\<tturnstile> cd \<leadsto>\<^sub>h) \<Sigma>\<^sub>h \<Sigma>\<^sub>h'' \<and> \<Sigma>\<^sub>b'' = unheap \<Sigma>\<^sub>h''" by fastforce
+  ultimately obtain \<Sigma>\<^sub>h'' where "iter (\<tturnstile> \<C> \<leadsto>\<^sub>h) \<Sigma>\<^sub>h' \<Sigma>\<^sub>h'' \<and> \<Sigma>\<^sub>b'' = unheap \<Sigma>\<^sub>h''" by blast
+  with S have "iter (\<tturnstile> \<C> \<leadsto>\<^sub>h) \<Sigma>\<^sub>h \<Sigma>\<^sub>h'' \<and> \<Sigma>\<^sub>b'' = unheap \<Sigma>\<^sub>h''" by fastforce
   thus ?case by fastforce
 qed force+
 
